test/openssl_echo_server.c
@@ -78,14 +78,12 @@ int main(int argc, char **argv) {
       SSL_CTX_set_max_proto_version(ctx, TLS1_3_VERSION) != 1 ||
       SSL_CTX_set_ciphersuites(ctx, "TLS_CHACHA20_POLY1305_SHA256") != 1 ||
       SSL_CTX_set1_groups_list(ctx, "X25519") != 1 ||
-      SSL_CTX_set_num_tickets(ctx, 0) != 1 ||
       SSL_CTX_use_certificate_file(ctx, argv[2], SSL_FILETYPE_PEM) != 1 ||
       SSL_CTX_use_PrivateKey_file(ctx, argv[3], SSL_FILETYPE_PEM) != 1 ||
       SSL_CTX_check_private_key(ctx) != 1) {
     ERR_print_errors_fp(stderr);
     goto done;
   }
-  SSL_CTX_set_session_cache_mode(ctx, SSL_SESS_CACHE_OFF);
   SSL_CTX_set_verify(ctx, SSL_VERIFY_NONE, NULL);
 
   uint16_t actual_port = 0;
