src/impl/TLS13.Impl.Messages.fst
@@ -131,6 +131,7 @@ type tls_message =
   | LTlsApplicationData of application_data
   | LTlsAlert of U8.t
   | LTlsChangeCipherSpec
+  | LTlsIgnoredPostHandshake of application_data
 
 let tls_message_is_handshake (l:tls_message) : bool =
   match l with
@@ -152,18 +153,25 @@ let tls_message_is_change_cipher_spec (l:tls_message) : bool =
   | LTlsChangeCipherSpec -> true
   | _ -> false
 
+let tls_message_is_ignored_post_handshake (l:tls_message) : bool =
+  match l with
+  | LTlsIgnoredPostHandshake _ -> true
+  | _ -> false
+
 let lemma_tls_message_classifier_complete (l:tls_message)
   : Lemma (
       tls_message_is_handshake l \/
       tls_message_is_application_data l \/
       tls_message_is_alert l \/
-      tls_message_is_change_cipher_spec l)
+      tls_message_is_change_cipher_spec l \/
+      tls_message_is_ignored_post_handshake l)
   =
   match l with
   | LTlsHandshake _ -> ()
   | LTlsApplicationData _ -> ()
   | LTlsAlert _ -> ()
   | LTlsChangeCipherSpec -> ()
+  | LTlsIgnoredPostHandshake _ -> ()
 
 noeq
 type tls_record = {
@@ -543,6 +551,8 @@ let is_valid_tls_message ([@@@mkey] l:tls_message) (m:M.tls_message) : slprop =
     exists* malert. pure (alert_description_matches lalert malert /\ m == M.TlsAlert malert)
   | LTlsChangeCipherSpec ->
     pure (m == M.TlsChangeCipherSpec)
+  | LTlsIgnoredPostHandshake lignored ->
+    exists* body. is_valid_application_data lignored body ** pure (m == M.TlsIgnoredPostHandshake body)
 
 let is_valid_tls_record ([@@@mkey] l:tls_record) (m:M.tls_record) : slprop =
   is_valid_sealed_record l.tls_record_fragment m.M.record_fragment **
@@ -684,6 +694,11 @@ fn free_tls_message
       unfold (is_valid_tls_message (LTlsApplicationData lapp) m);
       with mapp. _;
       free_application_data lapp
+    }
+    LTlsIgnoredPostHandshake lignored -> {
+      unfold (is_valid_tls_message (LTlsIgnoredPostHandshake lignored) m);
+      with body. _;
+      free_application_data lignored
     }
     LTlsAlert lalert -> {
       unfold (is_valid_tls_message (LTlsAlert lalert) m);
